"exact" maps as the base case of separation logic

src/coqutil/Map/Separation.v
@@ -2,11 +2,11 @@ Require Import coqutil.Map.Interface coqutil.Lift1Prop. Import map.
 
 Section Sep.
   Context {key value} {map : map key value}.
-  Definition emp (P : Prop) := fun m : map => m = empty /\ P.
   Definition sep (p q : map -> Prop) m :=
     exists mp mq, split m mp mq /\ p mp /\ q mq.
-  Definition ptsto k v := fun m : map => m = put empty k v.
-  Definition read k (P : value -> rep -> Prop) := (ex1 (fun v => sep (ptsto k v) (P v))).
+  Definition emp (P : Prop) := fun m : map => m = empty /\ P.
+  Definition exact (m : map) := Logic.eq m.
+  Definition ptsto k v : map -> Prop := exact (put empty k v).
 
   Fixpoint seps (xs : list (rep -> Prop)) : rep -> Prop :=
     match xs with
@@ -16,9 +16,17 @@ Section Sep.
     end.
 End Sep.
 
-Declare Scope sep_scope.
-Delimit Scope sep_scope with sep.
-Infix "*" := sep (at level 40, left associativity) : sep_scope.
-Infix "⋆" := sep (at level 40, left associativity) : sep_scope.
-Notation "m =* P" := ((P%sep) m) (at level 70, only parsing).
-Notation "m =*> P" := (exists R, (sep P R) m) (at level 70, only parsing).
+Module Export Notations.
+  Declare Scope sep_scope.
+  Delimit Scope sep_scope with sep.
+  Infix "*" := sep (at level 40, left associativity) : sep_scope.
+  Infix "⋆" := sep (at level 40, left associativity) : sep_scope.
+  Notation "m =* P" := ((P%sep) m) (at level 70, only parsing).
+  Notation "m =*> P" := (exists R, (sep P R) m) (at level 70, only parsing).
+End Notations.
+
+Module Export Coercions.
+  Coercion exact : Interface.map.rep >-> Funclass.
+End Coercions.
+
+Hint Unfold exact : core.
